all in same file

src/AlgebraBigraphs.v
@@ -1,232 +1,605 @@
-  From Coq Require Import Arith ZArith Psatz Bool
-                          String List Program.Equality Program.Wf.
-  Require Import Relations.
-  Require Import Recdef.
+From Coq Require Import Arith ZArith Psatz Bool
+                        String List Program.Equality Program.Wf.
+Require Import Relations.
+Require Import Recdef.
 
-  Require Import OrderedType.
-
-  Require Export Coq.FSets.FMapInterface.
+Require Import OrderedType.
 
 
 
-  Set Warnings "-parsing".
-  Unset Strict Implicit.
-  Unset Printing Implicit Defensive.
-  Set Warnings "parsing".
+Set Warnings "-parsing".
+Unset Strict Implicit.
+Unset Printing Implicit Defensive.
+Set Warnings "parsing".
 
-  Local Open Scope string_scope.
-  Local Open Scope list_scope.
-  Local Open Scope nat_scope.
-  Local Open Scope bool_scope.
-  Import ListNotations.
+Local Open Scope string_scope.
+Local Open Scope list_scope.
+Local Open Scope nat_scope.
+Local Open Scope bool_scope.
+Import ListNotations.
+
+Set Implicit Arguments.
 
 
-  Require Export Bool DecidableType OrderedType.
-  Set Implicit Arguments.
+Require Import FMapInterface.
 
-  Module Export MyBigraph.
 
-  Section Bigraphs.
 
+Module Type IdDec.
+
+Parameter A : Type.
+Parameter eq_decA : forall (a1 a2 : A), {a1 = a2} + {~ a1 = a2}.
+
+End IdDec.
+
+
+
+Module MyBigraph.
   Variable A : Type.
 
-  Inductive option {A:Type} : Type :=
-    | Some : A -> option
+  Inductive option {type:Type} : Type :=
+    | Some : type -> option
     | None : option.
 
-    Variant id (A:Type) : Type := 
-      Id : A -> id A. 
+  Variant id (A:Type) : Type := 
+    Id : A -> id A. 
 
-    Variant root : Type := 
-      Root : id A -> root.  
+  Variant root : Type := 
+    Root : id A -> root.  
 
-    Variant node  : Type := 
-      Node :  id A -> node.
+  Variant node (A:Type) : Type := 
+    Node :  id A -> node A.
 
-    Variant site  : Type := 
-      Site :  id A -> site. 
+  Module NodeProperties (IDDD : IdDec).
 
-    Variant place  : Type := 
-      | PRoot (r : root)
-      | PNode (n : node)
-      | PSite (s : site).
+    Definition A := IDDD.A.
+    Definition eq_decA := IDDD.eq_decA.
+  
+    Definition getIdNode (n : node A) : A :=
+      match n with Node (Id idn) => idn 
+      end.
+  
+    Definition eq_nodes (n1 n2 : node A) : Prop :=
+        getIdNode n1 = getIdNode n2.
     
-    Variant nors  : Type := 
-      | Ssite : site -> nors
-      | Snode : node -> nors.
+    Definition eq_nodes_dec: forall (n1 n2 : node A),
+      { getIdNode n1 = getIdNode n2 } + { ~ getIdNode n1 = getIdNode n2 }.
+      intros. destruct n1 as [a1], n2 as [a2].
+      destruct (eq_decA (getIdNode (Node a1)) (getIdNode (Node a2))); [left | right].
+      - apply e.
+      - apply n.
+    Defined.
+  
+    Definition eq_nodes_b (n1:node A) (n2:node A) : bool.
+      destruct (eq_decA (getIdNode n1) (getIdNode n2)).
+      - exact true.
+      - exact false.
+      Defined.
+  
+    Theorem eqb_eq_dec_reflects : forall (n1 n2 : node A),
+      reflect (eq_nodes n1 n2) (eq_nodes_b n1 n2).
+    Proof.
+      intros. unfold eq_nodes_b.
+      destruct (eq_nodes_dec n1 n2) as [H1 | H2].
+      - destruct eq_decA as [h1 | h2].
+        + constructor. apply h1.
+        + constructor. apply h2.
+      - destruct eq_decA as [h1 | h2].
+        + constructor. apply h1.
+        + constructor. apply h2.
+    Qed.
+  
+    Lemma eq_nodes_refl : forall n : node A, 
+      eq_nodes n n.
+    Proof. intros. unfold eq_nodes. unfold getIdNode. reflexivity. Qed.   
+  
+    Lemma eq_nodes_sym : forall (n1 n2 : node A), 
+      eq_nodes n1 n2 -> eq_nodes n2 n1.
+    Proof. intros. unfold eq_nodes.
+    unfold eq_nodes in H. symmetry in H. apply H. Qed.   
+  
+    Lemma eq_nodes_trans : forall (n1 n2 n3: node A), 
+      ((eq_nodes n1 n2) /\ (eq_nodes n2 n3)) -> (eq_nodes n1 n3).
+    Proof. intros. unfold eq_nodes. 
+    unfold eq_nodes in H. destruct H as [H1 H2].
+    rewrite H1. rewrite H2. reflexivity. Qed.   
+  
+  
+    (* Fixpoint getk {A:Type} (n:node A) (c:control A) : option :=
+      match c with 
+        | [] => None
+        | (n', idk, k) :: q => if (eq_nodes_b n n') then Some k else getk n q
+      end. 
+  
+  
+    Example k_v0: getk v0 mybig = Some 2.
+    Proof. unfold getk. unfold getctrl. simpl. reflexivity. Qed.
+    Example k_v1: getk v1 mybig = Some 2.
+    Proof. unfold getk. unfold getctrl. simpl. reflexivity. Qed.
+    Example k_v2: getk v2 mybig = Some 4.
+    Proof. unfold getk. unfold getctrl. simpl. reflexivity. Qed.
+  
+    Fixpoint count_links_to_node {A: Type} (n:node A) (b:bigraph A) :=
+      0. *)
+  
+  End NodeProperties.
 
-    Variant norr  : Type := 
-      | Rroot : root -> norr
-      | Rnode : node -> norr.
 
-    Variant outername  : Type := 
-      Outername :  id A -> outername. 
 
-    Variant innername  : Type := 
-      Innername :  id A -> innername.
 
-    Variant edge  : Type := 
-      Edge :  id A -> edge. 
+  Variant site  : Type := 
+    Site :  id A -> site. 
 
-    Variant port  : Type := 
-      Port : node -> nat -> port.
+  Variant place  : Type := 
+    | PRoot (r : root)
+    | PNode (n : node A)
+    | PSite (s : site).
+  
+  Variant nors  : Type := 
+    | Ssite : site -> nors
+    | Snode : node A -> nors.
 
-    Variant link  : Type := 
-      | Ledge: edge -> link
-      | Loutername : outername -> link.
+  Variant norr  : Type := 
+    | Rroot : root -> norr
+    | Rnode : node A -> norr.
 
-    Variant point  : Type := 
-      | Pport : port -> point
-      | Pinnername : innername -> point.
+  Variant outername  : Type := 
+    Outername :  id A -> outername. 
 
-    Definition control  : Type := node -> (id A * nat).
-    Definition parent  : Type := list (nors *  norr).
-    Definition link_m  : Type := list (point * link).
+  Variant innername  : Type := 
+    Innername :  id A -> innername.
 
-    Variant linkgraph  : Type :=
-      Linkgraph 
-        (v : list node)  
-        (e : list edge) 
-        (ctrl : control) 
-        (lnk : link_m)
-        (x : list innername) 
-        (y : list outername).
+  Variant edge  : Type := 
+    Edge :  id A -> edge. 
 
-    Variant placegraph {A:Type}: Type :=
-      Placegraph 
-        (v : list node)  
-        (ctrl : control) 
-        (prnt : parent) 
-        (m : list site) 
-        (n : list root).
+  Variant port  : Type := 
+    Port : node A -> nat -> port.
 
-    Inductive bigraph: Type :=
-      Bigraph 
-        (v : list node )  
-        (e : list edge) 
-        (ctrl : control) 
-        (prnt : parent) 
-        (lnk : link_m)
-        (m : list site) 
-        (n : list root)
-        (x : list innername) 
-        (y : list outername).
+  Variant link  : Type := 
+    | Ledge: edge -> link
+    | Loutername : outername -> link.
 
-    Definition getv (b:bigraph) : list node :=
-      match b with
-      | Bigraph v _ _ _ _ _ _ _ _ => v
-      end.
+  Variant point  : Type := 
+    | Pport : port -> point
+    | Pinnername : innername -> point.
 
-    Definition gete (b:bigraph) : list edge :=
-      match b with
-      | Bigraph _ e _ _ _ _ _ _ _ => e
-      end.
+  (****** SECTION ON MAPS ******)
+    Definition key : Type := node A.
+    Definition elt : Type := id A * nat.
+    Definition t (e:Type) : Type := list (node A * e).
+  (****** END SECTION ON MAPS ******)
 
-    Definition getctrl (b:bigraph) : control :=
-      match b with
-      | Bigraph _ _ ctrl _ _ _ _ _ _ => ctrl
-      end.
+  Definition control : Type := t elt.
+  Definition parent  : Type := list (nors *  norr).
+  Definition link_m  : Type := list (point * link).
+  Definition empty_control : control := [].
 
-    Definition getprnt (b:bigraph) : parent :=
-      match b with
-      | Bigraph _ _ _ prnt _ _ _ _ _ => prnt
-      end.
+  Variant linkgraph  : Type :=
+    Linkgraph 
+      (v : list (node A))  
+      (e : list edge) 
+      (ctrl : control) 
+      (lnk : link_m)
+      (x : list innername) 
+      (y : list outername).
 
-    Definition getlnk (b:bigraph) : link_m :=
-      match b with
-      | Bigraph _ _ _ _ lnk _ _ _ _ => lnk
-      end.
+  Variant placegraph {A:Type}: Type :=
+    Placegraph 
+      (v : list (node A))  
+      (ctrl : control) 
+      (prnt : parent) 
+      (m : list site) 
+      (n : list root).
 
-    Definition getm (b:bigraph) : list site :=
-      match b with
-      | Bigraph _ _ _ _ _ m _ _ _ => m
-      end.
+  Inductive bigraph: Type :=
+    Bigraph 
+      (v : list (node A) )  
+      (e : list edge) 
+      (ctrl : control) 
+      (prnt : parent) 
+      (lnk : link_m)
+      (m : list site) 
+      (n : list root)
+      (x : list innername) 
+      (y : list outername).
 
-    Definition getn (b:bigraph) : list root :=
-      match b with
-      | Bigraph _ _ _ _ _ _ n _ _ => n
-      end.
+  Definition getv (b:bigraph) : list (node A) :=
+    match b with
+    | Bigraph v _ _ _ _ _ _ _ _ => v
+    end.
 
-    Definition getx (b:bigraph) : list innername :=
-      match b with
-      | Bigraph _ _ _ _ _ _ _ x _ => x
-      end.
+  Definition gete (b:bigraph) : list edge :=
+    match b with
+    | Bigraph _ e _ _ _ _ _ _ _ => e
+    end.
 
-    Definition gety (b:bigraph) : list outername :=
-      match b with
-      | Bigraph _ _ _ _ _ _ _ _ y => y
-      end.
+  Definition getctrl (b:bigraph) : control :=
+    match b with
+    | Bigraph _ _ ctrl _ _ _ _ _ _ => ctrl
+    end.
 
-    End Bigraphs.
+  Definition getprnt (b:bigraph) : parent :=
+    match b with
+    | Bigraph _ _ _ prnt _ _ _ _ _ => prnt
+    end.
 
-    (* Example *)
-  Section testBigraph.
+  Definition getlnk (b:bigraph) : link_m :=
+    match b with
+    | Bigraph _ _ _ _ lnk _ _ _ _ => lnk
+    end.
 
-    Example v0 := Node (Id "v0").
-    Example v1 := Node (Id "v1").
-    Example v2 := Node (Id "v2").
+  Definition getm (b:bigraph) : list site :=
+    match b with
+    | Bigraph _ _ _ _ _ m _ _ _ => m
+    end.
 
-    Example x0 := Innername (Id "x0").
-    Example x1 := Innername (Id "x1").
+  Definition getn (b:bigraph) : list root :=
+    match b with
+    | Bigraph _ _ _ _ _ _ n _ _ => n
+    end.
 
-    Example y0 := Outername (Id "y0").
-    Example y1 := Outername (Id "y1").
-    Example y2 := Outername (Id "y2").
+  Definition getx (b:bigraph) : list innername :=
+    match b with
+    | Bigraph _ _ _ _ _ _ _ x _ => x
+    end.
 
-    Example e0 := Edge  (Id "e0").
-    Example e1 := Edge  (Id "e1").
-    Example e2 := Edge  (Id "e2").
-    Example e3 := Edge  (Id "e3").
-    Example e4 := Edge  (Id "e4").
+  Definition gety (b:bigraph) : list outername :=
+    match b with
+    | Bigraph _ _ _ _ _ _ _ _ y => y
+    end.
 
-    Example ctrltest (v:node string) := match v with 
-      | Node (Id "v0") => (Id "K", 2) 
-      | Node (Id "v1") => (Id "K", 2) 
-      | Node (Id "v2") => (Id "M", 4)
-      | _ => (Id "_", 0) (*weird case*)
-      end.
-
-    (* Check ctrltest : control string. *)
-
-    Example site0 := Site (Id "s0").
-    Example site1 := Site (Id "s1").
-      
-    Example root0 := Root (Id "r0").
-    Example root1 := Root (Id "r1").
-
-    Example prnttest :=
-      [ (Snode v0, Rroot root0); 
-        (Snode v1, Rnode v0); 
-        (Snode v2, Rroot root1);
-        (Ssite site0, Rnode v0);
-        (Ssite site1, Rnode v2)].
-
-    Example lnktest :=
-      [ (Pport (Port v0 1) ,  Loutername y0);
-        (Pport (Port v0 2) ,  Ledge e0);
-        (Pport (Port v1 1) ,  Loutername y0);
-        (Pport (Port v1 2) ,  Ledge e1);
-        (Pport (Port v2 1) ,  Loutername y1);
-        (Pport (Port v2 2) ,  Loutername y2);
-        (Pport (Port v2 3) ,  Ledge e0);
-        (Pport (Port v2 4) ,  Ledge e1);
-        (Pinnername x0, Ledge e0);
-        (Pinnername x1, Loutername y2)].
-
-    Example mybig :=  
-      Bigraph
-        [ v0 ;  v1 ; v2 ]
-        [ e0 ; e1 ; e2; e3 ; e4]
-        ctrltest
-        prnttest 
-        lnktest
-        [ site0 ; site1 ]
-        [ root0 ; root1 ]
-        [ x0 ; x1 ]
-        [ y0 ; y1 ; y2 ].
-
-    (* Check mybig : bigraph string. *)
-
-  End testBigraph.
   End MyBigraph.
+
+  (* Example
+Section testBigraph.
+
+  Example v0 := Node (Id "v0").
+  Example v1 := Node (Id "v1").
+  Example v2 := Node (Id "v2").
+
+  Example x0 := Innername (Id "x0").
+  Example x1 := Innername (Id "x1").
+
+  Example y0 := Outername (Id "y0").
+  Example y1 := Outername (Id "y1").
+  Example y2 := Outername (Id "y2").
+
+  Example e0 := Edge  (Id "e0").
+  Example e1 := Edge  (Id "e1").
+  Example e2 := Edge  (Id "e2").
+  Example e3 := Edge  (Id "e3").
+  Example e4 := Edge  (Id "e4").
+
+  Example ctrltest : control string := 
+    empty_control string.
+  (* match v with 
+    | Node (Id "v0") => (Id "K", 2) 
+    | Node (Id "v1") => (Id "K", 2) 
+    | Node (Id "v2") => (Id "M", 4)
+    | _ => (Id "_", 0) (*weird case*)
+    end. *)
+
+  (* Check ctrltest : control string. *)
+
+  Example site0 := Site (Id "s0").
+  Example site1 := Site (Id "s1").
+    
+  Example root0 := Root (Id "r0").
+  Example root1 := Root (Id "r1").
+
+  Example prnttest :=
+    [ (Snode v0, Rroot root0); 
+      (Snode v1, Rnode v0); 
+      (Snode v2, Rroot root1);
+      (Ssite site0, Rnode v0);
+      (Ssite site1, Rnode v2)].
+
+  Example lnktest :=
+    [ (Pport (Port v0 1) ,  Loutername y0);
+      (Pport (Port v0 2) ,  Ledge e0);
+      (Pport (Port v1 1) ,  Loutername y0);
+      (Pport (Port v1 2) ,  Ledge e1);
+      (Pport (Port v2 1) ,  Loutername y1);
+      (Pport (Port v2 2) ,  Loutername y2);
+      (Pport (Port v2 3) ,  Ledge e0);
+      (Pport (Port v2 4) ,  Ledge e1);
+      (Pinnername x0, Ledge e0);
+      (Pinnername x1, Loutername y2)].
+
+  Example mybig :=  
+    Bigraph
+      [ v0 ;  v1 ; v2 ]
+      [ e0 ; e1 ; e2; e3 ; e4]
+      ctrltest
+      prnttest 
+      lnktest
+      [ site0 ; site1 ]
+      [ root0 ; root1 ]
+      [ x0 ; x1 ]
+      [ y0 ; y1 ; yVariant id (a:A) : Type := 
+    Id : a -> id A. 
+
+  Variant root : Type := 
+    Root : id A -> root.  
+
+  Variant node  : Type := 
+    Node :  id A -> node.
+
+  Module NodeProperties (IDD : IdDec).
+    Import IDD.
+    Definition A := IDD.A.
+  
+    Definition getIdNode (n : node A) : A :=
+      match n with Node (Id idn) => idn 
+      end.
+  
+    Definition eq_nodes (n1 n2:node A) : Prop :=
+        getIdNode n1 = getIdNode n2.
+    
+    Definition eq_nodes_dec: forall (n1 n2 : node A),
+      { getIdNode n1 = getIdNode n2 } + { ~ getIdNode n1 = getIdNode n2 }.
+      intros. destruct n1 as [a1], n2 as [a2].
+      destruct (eq_decA (getIdNode (Node a1)) (getIdNode (Node a2))); [left | right].
+      - apply e.
+      - apply n.
+    Defined.
+  
+    Definition eq_nodes_b (n1:node A) (n2:node A) : bool.
+      destruct (eq_decA (getIdNode n1) (getIdNode n2)).
+      - exact true.
+      - exact false.
+      Defined.
+  
+    Theorem eqb_eq_dec_reflects : forall (n1 n2 : node A),
+      reflect (eq_nodes n1 n2) (eq_nodes_b n1 n2).
+    Proof.
+      intros. unfold eq_nodes_b.
+      destruct (eq_nodes_dec n1 n2) as [H1 | H2].
+      - destruct eq_decA as [h1 | h2].
+        + constructor. apply h1.
+        + constructor. apply h2.
+      - destruct eq_decA as [h1 | h2].
+        + constructor. apply h1.
+        + constructor. apply h2.
+    Qed.
+  
+    Lemma eq_nodes_refl : forall n : node A, 
+      eq_nodes n n.
+    Proof. intros. unfold eq_nodes. unfold getIdNode. reflexivity. Qed.   
+  
+    Lemma eq_nodes_sym : forall (n1 n2 : node A), 
+      eq_nodes n1 n2 -> eq_nodes n2 n1.
+    Proof. intros. unfold eq_nodes.
+    unfold eq_nodes in H. symmetry in H. apply H. Qed.   
+  
+    Lemma eq_nodes_trans : forall (n1 n2 n3: node A), 
+      ((eq_nodes n1 n2) /\ (eq_nodes n2 n3)) -> (eq_nodes n1 n3).
+    Proof. intros. unfold eq_nodes. 
+    unfold eq_nodes in H. destruct H as [H1 H2].
+    rewrite H1. rewrite H2. reflexivity. Qed.   
+  
+  
+    (* Fixpoint getk {A:Type} (n:node A) (c:control A) : option :=
+      match c with 
+        | [] => None
+        | (n', idk, k) :: q => if (eq_nodes_b n n') then Some k else getk n q
+      end. 
+  
+  
+    Example k_v0: getk v0 mybig = Some 2.
+    Proof. unfold getk. unfold getctrl. simpl. reflexivity. Qed.
+    Example k_v1: getk v1 mybig = Some 2.
+    Proof. unfold getk. unfold getctrl. simpl. reflexivity. Qed.
+    Example k_v2: getk v2 mybig = Some 4.
+    Proof. unfold getk. unfold getctrl. simpl. reflexivity. Qed.
+  
+    Fixpoint count_links_to_node {A: Type} (n:node A) (b:bigraph A) :=
+      0. *)
+  
+  End Properties.
+
+
+
+
+  Variant site  : Type := 
+    Site :  id A -> site. 
+
+  Variant place  : Type := 
+    | PRoot (r : root)
+    | PNode (n : node)
+    | PSite (s : site).
+  
+  Variant nors  : Type := 
+    | Ssite : site -> nors
+    | Snode : node -> nors.
+
+  Variant norr  : Type := 
+    | Rroot : root -> norr
+    | Rnode : node -> norr.
+
+  Variant outername  : Type := 
+    Outername :  id A -> outername. 
+
+  Variant innername  : Type := 
+    Innername :  id A -> innername.
+
+  Variant edge  : Type := 
+    Edge :  id A -> edge. 
+
+  Variant port  : Type := 
+    Port : node -> nat -> port.
+
+  Variant link  : Type := 
+    | Ledge: edge -> link
+    | Loutername : outername -> link.
+
+  Variant point  : Type := 
+    | Pport : port -> point
+    | Pinnername : innername -> point.
+
+  (****** SECTION ON MAPS ******)
+    Definition key : Type := node.
+    Definition elt : Type := id A * nat.
+    Definition t (e:Type) : Type := list (node * e).
+  (****** END SECTION ON MAPS ******)
+
+  Definition control : Type := t elt.
+  Definition parent  : Type := list (nors *  norr).
+  Definition link_m  : Type := list (point * link).
+  Definition empty_control : control := [].
+
+  Variant linkgraph  : Type :=
+    Linkgraph 
+      (v : list node)  
+      (e : list edge) 
+      (ctrl : control) 
+      (lnk : link_m)
+      (x : list innername) 
+      (y : list outername).
+
+  Variant placegraph {A:Type}: Type :=
+    Placegraph 
+      (v : list node)  
+      (ctrl : control) 
+      (prnt : parent) 
+      (m : list site) 
+      (n : list root).
+
+  Inductive bigraph: Type :=
+    Bigraph 
+      (v : list node )  
+      (e : list edge) 
+      (ctrl : control) 
+      (prnt : parent) 
+      (lnk : link_m)
+      (m : list site) 
+      (n : list root)
+      (x : list innername) 
+      (y : list outername).
+
+  Definition getv (b:bigraph) : list node :=
+    match b with
+    | Bigraph v _ _ _ _ _ _ _ _ => v
+    end.
+
+  Definition gete (b:bigraph) : list edge :=
+    match b with
+    | Bigraph _ e _ _ _ _ _ _ _ => e
+    end.
+
+  Definition getctrl (b:bigraph) : control :=
+    match b with
+    | Bigraph _ _ ctrl _ _ _ _ _ _ => ctrl
+    end.
+
+  Definition getprnt (b:bigraph) : parent :=
+    match b with
+    | Bigraph _ _ _ prnt _ _ _ _ _ => prnt
+    end.
+
+  Definition getlnk (b:bigraph) : link_m :=
+    match b with
+    | Bigraph _ _ _ _ lnk _ _ _ _ => lnk
+    end.
+
+  Definition getm (b:bigraph) : list site :=
+    match b with
+    | Bigraph _ _ _ _ _ m _ _ _ => m
+    end.
+
+  Definition getn (b:bigraph) : list root :=
+    match b with
+    | Bigraph _ _ _ _ _ _ n _ _ => n
+    end.
+
+  Definition getx (b:bigraph) : list innername :=
+    match b with
+    | Bigraph _ _ _ _ _ _ _ x _ => x
+    end.
+
+  Definition gety (b:bigraph) : list outername :=
+    match b with
+    | Bigraph _ _ _ _ _ _ _ _ y => y
+    end.
+
+  End Bigraphs.
+
+  (* Example
+Section testBigraph.
+
+  Example v0 := Node (Id "v0").
+  Example v1 := Node (Id "v1").
+  Example v2 := Node (Id "v2").
+
+  Example x0 := Innername (Id "x0").
+  Example x1 := Innername (Id "x1").
+
+  Example y0 := Outername (Id "y0").
+  Example y1 := Outername (Id "y1").
+  Example y2 := Outername (Id "y2").
+
+  Example e0 := Edge  (Id "e0").
+  Example e1 := Edge  (Id "e1").
+  Example e2 := Edge  (Id "e2").
+  Example e3 := Edge  (Id "e3").
+  Example e4 := Edge  (Id "e4").
+
+  Example ctrltest : control string := 
+    empty_control string.
+  (* match v with 
+    | Node (Id "v0") => (Id "K", 2) 
+    | Node (Id "v1") => (Id "K", 2) 
+    | Node (Id "v2") => (Id "M", 4)
+    | _ => (Id "_", 0) (*weird case*)
+    end. *)
+
+  (* Check ctrltest : control string. *)
+
+  Example site0 := Site (Id "s0").
+  Example site1 := Site (Id "s1").
+    
+  Example root0 := Root (Id "r0").
+  Example root1 := Root (Id "r1").
+
+  Example prnttest :=
+    [ (Snode v0, Rroot root0); 
+      (Snode v1, Rnode v0); 
+      (Snode v2, Rroot root1);
+      (Ssite site0, Rnode v0);
+      (Ssite site1, Rnode v2)].
+
+  Example lnktest :=
+    [ (Pport (Port v0 1) ,  Loutername y0);
+      (Pport (Port v0 2) ,  Ledge e0);
+      (Pport (Port v1 1) ,  Loutername y0);
+      (Pport (Port v1 2) ,  Ledge e1);
+      (Pport (Port v2 1) ,  Loutername y1);
+      (Pport (Port v2 2) ,  Loutername y2);
+      (Pport (Port v2 3) ,  Ledge e0);
+      (Pport (Port v2 4) ,  Ledge e1);
+      (Pinnername x0, Ledge e0);
+      (Pinnername x1, Loutername y2)].
+
+  Example mybig :=  
+    Bigraph
+      [ v0 ;  v1 ; v2 ]
+      [ e0 ; e1 ; e2; e3 ; e4]
+      ctrltest
+      prnttest 
+      lnktest
+      [ site0 ; site1 ]
+      [ root0 ; root1 ]
+      [ x0 ; x1 ]
+      [ y0 ; y1 ; y2 ].
+
+  (* Check mybig : bigraph string. *)
+
+End testBigraph. *)
+End MyBigraph.
+2 ].
+
+  (* Check mybig : bigraph string. *)
+
+End testBigraph. *)
+
 
